src/test.sh
@@ -10,5 +10,9 @@ $main find-word 32
 echo 
 $main word-verification 32
 echo 
+$main init-rtl-state
+echo 
+$main instruction-verification-proposition
+echo 
 $main instruction-verification
 
